towards a better spec for increment
Needed to admit many properties about read-after-write.

examples/low-level/example1.fst
@@ -24,3 +24,7 @@ val increment : r:(ref int) -> SST unit  (fun m -> (refExistsInMem r m)==true) (
 let increment r =
   let oldv = read r in
   write r (oldv + 1)
+
+(*ideally, the refExistsInMem clauses should not be needed in the postcondition*)
+val increment2 : r:(ref int) -> SST unit  (fun m -> (refExistsInMem r m)==true) (fun m0 a m1 -> (refExistsInMem r m0) /\ (refExistsInMem r m1) /\ (loopkupRef r m1 = (loopkupRef r m0) + 1))
+let increment2 r = admit ()
